secure_api/box/functor_box/Box.PKAE.fst
@@ -1,0 +1,84 @@
+(**
+  This module represents the PKAE cryptographic security game expressed in terms of the underlying cryptobox construction.
+*)
+module Box.PKAE
+
+
+open FStar.Set
+open FStar.HyperHeap
+open FStar.HyperStack
+open FStar.HyperStack.ST
+open FStar.Monotonic.RRef
+open FStar.Seq
+open FStar.Monotonic.Seq
+open FStar.List.Tot
+
+open Crypto.Symmetric.Bytes
+
+open Box.Flags
+
+module MR = FStar.Monotonic.RRef
+module MM = MonotoneMap
+module HS = FStar.HyperStack
+module HH = FStar.HyperHeap
+module HSalsa = Spec.HSalsa20
+module Curve = Spec.Curve25519
+module SPEC = Spec.SecretBox
+module Plain = Box.Plain
+module Key = Box.Key
+module ID = Box.Indexing
+module ODH = Box.ODH
+module AE = Box.AE
+
+#set-options "--z3rlimit 1900 --max_ifuel 1 --max_fuel 0"
+abstract noeq type pkae_module =
+  | PKAE:
+    im:ID.index_module{ID.get_subId im == ODH.dh_share} ->
+    pm:Plain.plain_module{Plain.get_plain pm == AE.ae_plain} ->
+    am:AE.ae_module im pm ->
+    km:Key.key_module im{km == AE.instantiate_km am} ->
+    om:ODH.odh_module im km ->
+    pkae_module
+
+type skey = ODH.skey
+type pkey = ODH.pkey
+type nonce = AE.nonce
+type key (pkm:pkae_module) = AE.key pkm.im
+type id (pkm:pkae_module) = ID.id pkm.im
+type message (pkm:pkae_module) (i:id pkm) = AE.ae_protected_plain pkm.im pkm.pm i
+type cipher = AE.cipher
+
+val gen: pkm:pkae_module -> ST (pkey*skey)
+  (requires (fun h0 -> True))
+  (ensures (fun h0 _ h1 -> modifies_none h0 h1))
+let gen pkm =
+  ODH.keygen()
+
+let fresh pkm i = ID.fresh pkm.im (ID.ID i)
+let registered pkm i = ID.registered pkm.im (ID.ID i)
+let honest pkm i = ID.honest pkm.im (ID.ID i)
+let dishonest pkm i = ID.dishonest pkm.im (ID.ID i)
+
+#set-options "--z3rlimit 5000 --max_ifuel 2 --max_fuel 0"
+val encrypt: pkm:pkae_module -> #i:id pkm -> n:nonce -> sk:skey -> pk:pkey{ODH.compatible_keys sk pk /\ i = ID.compose_ids pkm.im (ODH.pk_get_share pk) (ODH.sk_get_share sk)} -> m:message pkm i{Plain.length #pkm.im #pkm.pm #i m / Spec.Salsa20.blocklen < pow2 32} -> ST cipher
+  (requires (fun h0 ->
+    registered pkm i
+    /\ AE.nonce_is_fresh pkm.am i n h0
+    /\ Key.km_invariant pkm.im pkm.km h0
+  ))
+  (ensures  (fun h0 c h1 ->
+    Key.km_invariant pkm.im pkm.km h1
+  ))
+let encrypt pkm #i n sk pk m =
+  let h0 = get() in
+  assert(Key.km_invariant pkm.im pkm.km h0);
+  let k = ODH.prf_odh pkm.im pkm.km pkm.om sk pk in
+  let h1 = get() in
+  assert(Key.km_invariant pkm.im pkm.km h1);
+  assert(Key.get_keytype pkm.im pkm.km == AE.key pkm.im);
+  let c = AE.encrypt pkm.am #i n k m in
+  c
+
+//
+//
+//val decrypt: pkm:pkae_module -> #i:id pkm -> n:nonce -> k:key pkm -> c:cipher -> option (message pkm i)
